pulse/ulib/experimental/Steel.Effect.fsti
@@ -450,26 +450,6 @@ val par (#aL:Type u#a)
     (fun h -> lpreL h /\ lpreR h)
     (fun h0 y h1 -> lpreL h0 /\ lpreR h0 /\ lpostL h0 (fst y) h1 /\ lpostR h0 (snd y) h1)
 
-val rewrite_context (#[@@@ framing_implicit] p:slprop)
-                    (#[@@@ framing_implicit] q:slprop)
-                    (_:unit)
-  : SteelF unit p (fun _ -> q) (requires fun _ -> p `equiv` q) (ensures fun _ _ _ -> True)
-
-val extract_info (p:slprop) (fact:prop)
-  (l:(m:mem) -> Lemma (requires interp p m) (ensures fact))
-  : Steel unit p (fun _ -> p)
-      (fun _ -> True)
-      (fun _ _ _ -> fact)
-
-val sladmit (#a:Type)
-            (#[@@@ framing_implicit] p:pre_t)
-            (#[@@@ framing_implicit] q:post_t a)
-            (_:unit)
-  : SteelF a p q (requires fun _ -> True) (ensures fun _ _ _ -> False)
-
-val intro_pure (p:prop)
-  : Steel unit emp (fun _ -> pure p) (requires fun _ -> p) (ensures fun _ _ _ -> True)
-
 val read (#a:Type)
          (#pcm:_)
          (r:ref a pcm)
@@ -549,7 +529,6 @@ val cond (#a:Type)
          (then_: (squash (b == true) -> SteelT a (p true) (q true)))
          (else_: (squash (b == false) -> SteelT a (p false) (q false)))
   : SteelT a (p b) (q b)
-
 
 val drop (p:slprop) : SteelT unit p (fun _ -> emp)
 
